update components & casting

ArkLib/OracleReduction/Cast.lean
@@ -20,97 +20,120 @@ import ArkLib.OracleReduction.Security.Basic
 
 namespace ProtocolSpec
 
-variable {m n : ℕ} (h : m = n)
+variable {n₁ n₂ : ℕ} (hn : n₁ = n₂)
 
 /-! ### Casting Protocol Specifications -/
 
 /-- Casting a `ProtocolSpec` across an equality of the number of rounds
 
 One should use the type-class function `dcast` instead of this one. -/
-protected def cast (pSpec : ProtocolSpec m) : ProtocolSpec n :=
-  pSpec ∘ (Fin.cast h.symm)
+protected def cast (pSpec : ProtocolSpec n₁) : ProtocolSpec n₂ :=
+  pSpec ∘ (Fin.cast hn.symm)
 
 @[simp]
-theorem cast_id : ProtocolSpec.cast (Eq.refl m) = id := rfl
+theorem cast_id : ProtocolSpec.cast (Eq.refl n₁) = id := rfl
 
 instance instDCast : DCast Nat ProtocolSpec where
   dcast h := ProtocolSpec.cast h
   dcast_id := cast_id
 
-theorem cast_eq_dcast {h : m = n} {pSpec : ProtocolSpec m} :
+theorem cast_eq_dcast {h : n₁ = n₂} {pSpec : ProtocolSpec n₁} :
     pSpec.cast h = dcast h pSpec := rfl
 
 /-! ### Casting (Partial) Transcripts -/
 
-variable {pSpec₁ : ProtocolSpec m} {pSpec₂ : ProtocolSpec n}
+variable {pSpec₁ : ProtocolSpec n₁} {pSpec₂ : ProtocolSpec n₂}
 
 @[simp]
-theorem cast_funext {h} (hSpec : pSpec₁.cast h = pSpec₂) {i : Fin n} :
-    pSpec₁ (Fin.cast h.symm i) = pSpec₂ i := funext_iff.mp hSpec i
+theorem cast_idx (hSpec : pSpec₁.cast hn = pSpec₂) {i : Fin n₁} :
+    pSpec₂ (Fin.cast hn i) = pSpec₁ i := by
+  simp [← hSpec, ProtocolSpec.cast]
 
-alias cast_idx := cast_funext
+@[simp]
+theorem cast_idx_symm {hn} (hSpec : pSpec₁.cast hn = pSpec₂) {i : Fin n₂} :
+    pSpec₁ (Fin.cast hn.symm i) = pSpec₂ i := funext_iff.mp hSpec i
 
-theorem cast_symm {h} (hSpec : pSpec₁.cast h = pSpec₂) : pSpec₂.cast h.symm = pSpec₁ := by
+theorem cast_symm {hn} (hSpec : pSpec₁.cast hn = pSpec₂) : pSpec₂.cast hn.symm = pSpec₁ := by
   rw [cast_eq_dcast] at hSpec ⊢
-  exact dcast_symm h hSpec
+  exact dcast_symm hn hSpec
 
-variable (hSpec : pSpec₁.cast h = pSpec₂)
+variable (hSpec : pSpec₁.cast hn = pSpec₂)
 
 namespace MessageIdx
 
 /-- Casting a message index across an equality of `ProtocolSpec`s. -/
 protected def cast (i : MessageIdx pSpec₁) : MessageIdx pSpec₂ :=
-  ⟨Fin.cast h i.1, by simp [← hSpec, ProtocolSpec.cast, i.property]⟩
+  ⟨Fin.cast hn i.1, by simp [← hSpec, ProtocolSpec.cast, i.property]⟩
 
 @[simp]
-theorem cast_id : MessageIdx.cast (Eq.refl m) rfl = (id : pSpec₁.MessageIdx → _) := rfl
+theorem cast_id : MessageIdx.cast (Eq.refl n₁) rfl = (id : pSpec₁.MessageIdx → _) := rfl
+
+theorem cast_injective : Function.Injective (MessageIdx.cast hn hSpec) := by
+  intro i j h'
+  simp [MessageIdx.cast] at h'
+  ext : 1
+  exact h'
 
 instance instDCast₂ : DCast₂ Nat ProtocolSpec (fun _ pSpec => MessageIdx pSpec) where
   dcast₂ h := MessageIdx.cast h
   dcast₂_id := cast_id
 
-theorem cast_eq_dcast₂ {h} {hSpec : pSpec₁.cast h = pSpec₂} {i : MessageIdx pSpec₁}:
-    i.cast h hSpec = dcast₂ h hSpec i := rfl
+theorem cast_eq_dcast₂ {hn} {hSpec : pSpec₁.cast hn = pSpec₂} {i : MessageIdx pSpec₁}:
+    i.cast hn hSpec = dcast₂ hn hSpec i := rfl
 
 end MessageIdx
 
+namespace Message
+
 @[simp]
-theorem Message.cast_idx {i : MessageIdx pSpec₂} :
-    pSpec₁.Message (i.cast h.symm (cast_symm hSpec)) = pSpec₂.Message i := by
+theorem cast_idx {i : MessageIdx pSpec₂} :
+    pSpec₁.Message (i.cast hn.symm (cast_symm hSpec)) = pSpec₂.Message i := by
   simp [MessageIdx.cast]
-  exact congrArg Prod.snd (cast_funext hSpec)
+  exact congrArg Prod.snd (cast_idx_symm hSpec)
+
+instance [inst : ∀ i, OracleInterface (pSpec₁.Message i)] :
+    ∀ i, OracleInterface ((pSpec₁.cast hn).Message i) :=
+  fun i => inst (dcast₂ hn.symm (by rw [dcast_symm hn]; rfl) i)
+
+end Message
 
 namespace ChallengeIdx
 
 /-- Casting a challenge index across an equality of `ProtocolSpec`s. -/
 protected def cast (i : ChallengeIdx pSpec₁) : ChallengeIdx pSpec₂ :=
-  ⟨Fin.cast h i.1, by simp [← hSpec, ProtocolSpec.cast, i.property]⟩
+  ⟨Fin.cast hn i.1, by simp [← hSpec, ProtocolSpec.cast, i.property]⟩
 
 @[simp]
-theorem cast_id : ChallengeIdx.cast (Eq.refl m) rfl = (id : pSpec₁.ChallengeIdx → _) := rfl
+theorem cast_id : ChallengeIdx.cast (Eq.refl n₁) rfl = (id : pSpec₁.ChallengeIdx → _) := rfl
+
+theorem cast_injective : Function.Injective (ChallengeIdx.cast hn hSpec) := by
+  intro i j h'
+  simp [ChallengeIdx.cast] at h'
+  ext : 1
+  exact h'
 
 instance instDCast₂ : DCast₂ Nat ProtocolSpec (fun _ pSpec => ChallengeIdx pSpec) where
   dcast₂ h := ChallengeIdx.cast h
   dcast₂_id := cast_id
 
-theorem cast_eq_dcast₂ {h : m = n} {hSpec : pSpec₁.cast h = pSpec₂} {i : ChallengeIdx pSpec₁}:
-    i.cast h hSpec = dcast₂ h hSpec i := rfl
+theorem cast_eq_dcast₂ {hn} {hSpec : pSpec₁.cast hn = pSpec₂} {i : ChallengeIdx pSpec₁}:
+    i.cast hn hSpec = dcast₂ hn hSpec i := rfl
 
 end ChallengeIdx
 
 @[simp]
 theorem Challenge.cast_idx {i : ChallengeIdx pSpec₂} :
-    pSpec₁.Challenge (i.cast h.symm (cast_symm hSpec)) = pSpec₂.Challenge i := by
+    pSpec₁.Challenge (i.cast hn.symm (cast_symm hSpec)) = pSpec₂.Challenge i := by
   simp [ChallengeIdx.cast]
-  exact congrArg Prod.snd (cast_funext hSpec)
+  exact congrArg Prod.snd (cast_idx_symm hSpec)
 
-variable {k : Fin (m + 1)} {l : Fin (n + 1)}
+variable {k : Fin (n₁ + 1)} {l : Fin (n₂ + 1)}
 
 namespace Transcript
 
 /-- Casting two partial transcripts across an equality of `ProtocolSpec`s, where the cutoff indices
   are equal. -/
-protected def cast (hIdx : k.val = l.val) (hSpec : pSpec₁.cast h = pSpec₂)
+protected def cast (hIdx : k.val = l.val) (hSpec : pSpec₁.cast hn = pSpec₂)
     (T : pSpec₁.Transcript k) : pSpec₂.Transcript l :=
   fun i => _root_.cast (by rw [← hSpec]; rfl) (T (Fin.cast hIdx.symm i))
 
@@ -140,7 +163,7 @@ namespace FullTranscript
 Internally invoke `Transcript.cast` with the last indices. -/
 protected def cast (T : FullTranscript pSpec₁) :
     FullTranscript pSpec₂ :=
-  Transcript.cast (k := Fin.last m) (l := Fin.last n) h h hSpec T
+  Transcript.cast (k := Fin.last n₁) (l := Fin.last n₂) hn hn hSpec T
 
 @[simp]
 theorem cast_id : FullTranscript.cast rfl rfl = (id : pSpec₁.FullTranscript → _) := rfl
@@ -150,38 +173,70 @@ instance instDCast₂ : DCast₂ Nat ProtocolSpec (fun _ pSpec => FullTranscript
   dcast₂_id := cast_id
 
 theorem cast_eq_dcast₂ {T : FullTranscript pSpec₁} :
-    dcast₂ h hSpec T = FullTranscript.cast h hSpec T := rfl
+    dcast₂ hn hSpec T = FullTranscript.cast hn hSpec T := rfl
 
 end FullTranscript
 
 end ProtocolSpec
 
-variable {ι : Type} {oSpec : OracleSpec ι} {StmtIn WitIn StmtOut WitOut : Type}
-variable {m n : ℕ} {pSpec₁ : ProtocolSpec m} {pSpec₂ : ProtocolSpec n}
-variable (h : m = n) (hSpec : pSpec₁.cast h = pSpec₂)
+variable {ι : Type} {oSpec : OracleSpec ι}
+  {StmtIn : Type} {ιₛᵢ : Type} {OStmtIn : ιₛᵢ → Type} [Oₛᵢ : ∀ i, OracleInterface (OStmtIn i)]
+  {WitIn : Type}
+  {StmtOut : Type} {ιₛₒ : Type} {OStmtOut : ιₛₒ → Type} [Oₛₒ : ∀ i, OracleInterface (OStmtOut i)]
+  {WitOut : Type}
+  {n₁ n₂ : ℕ} {pSpec₁ : ProtocolSpec n₁} {pSpec₂ : ProtocolSpec n₂}
+  (hn : n₁ = n₂) (hSpec : pSpec₁.cast hn = pSpec₂)
 
 open ProtocolSpec
-
-/-! ### Casting Provers -/
 
 namespace Prover
 
 /-- Casting the prover of a non-oracle reduction across an equality of `ProtocolSpec`s. -/
 protected def cast (P : Prover oSpec StmtIn WitIn StmtOut WitOut pSpec₁) :
     Prover oSpec StmtIn WitIn StmtOut WitOut pSpec₂ where
-  PrvState := P.PrvState ∘ Fin.cast (congrArg (· + 1) h.symm)
+  PrvState := P.PrvState ∘ Fin.cast (congrArg (· + 1) hn.symm)
   input := P.input
   sendMessage := fun i st => do
-    let ⟨msg, newSt⟩ ← P.sendMessage (i.cast h.symm (cast_symm hSpec)) st
-    return ⟨(Message.cast_idx h hSpec) ▸ msg, newSt⟩
+    let ⟨msg, newSt⟩ ← P.sendMessage (i.cast hn.symm (cast_symm hSpec)) st
+    return ⟨(Message.cast_idx hn hSpec) ▸ msg, newSt⟩
   receiveChallenge := fun i st => do
-    let f ← P.receiveChallenge (i.cast h.symm (cast_symm hSpec)) st
-    return fun chal => f (Challenge.cast_idx h hSpec ▸ chal)
+    let f ← P.receiveChallenge (i.cast hn.symm (cast_symm hSpec)) st
+    return fun chal => f (Challenge.cast_idx hn hSpec ▸ chal)
   output := P.output ∘ (fun st => _root_.cast (by simp) st)
+
+@[simp]
+theorem cast_id :
+    Prover.cast rfl rfl = (id : Prover oSpec StmtIn WitIn StmtOut WitOut pSpec₁ → _) := by
+  funext; simp [Prover.cast]; ext <;> simp; rfl
+
+instance instDCast₂ : DCast₂ Nat ProtocolSpec
+    (fun _ pSpec => Prover oSpec StmtIn WitIn StmtOut WitOut pSpec) where
+  dcast₂ := Prover.cast
+  dcast₂_id := Prover.cast_id
 
 end Prover
 
-/-! ### Casting Verifiers -/
+namespace OracleProver
+
+/-- Casting the oracle prover of a non-oracle reduction across an equality of `ProtocolSpec`s.
+
+Internally invokes the `Prover.cast` function. -/
+protected def cast (P : OracleProver oSpec StmtIn OStmtIn WitIn StmtOut OStmtOut WitOut pSpec₁) :
+    OracleProver oSpec StmtIn OStmtIn WitIn StmtOut OStmtOut WitOut pSpec₂ :=
+  Prover.cast hn hSpec P
+
+@[simp]
+theorem cast_id :
+    OracleProver.cast rfl rfl =
+      (id : OracleProver oSpec StmtIn OStmtIn WitIn StmtOut OStmtOut WitOut pSpec₁ → _) := by
+  sorry
+
+instance instDCast₂OracleProver : DCast₂ Nat ProtocolSpec
+    (fun _ pSpec => OracleProver oSpec StmtIn OStmtIn WitIn StmtOut OStmtOut WitOut pSpec) where
+  dcast₂ := OracleProver.cast
+  dcast₂_id := OracleProver.cast_id
+
+end OracleProver
 
 namespace Verifier
 
@@ -190,7 +245,7 @@ namespace Verifier
 This boils down to casting the (full) transcript. -/
 protected def cast (V : Verifier oSpec StmtIn StmtOut pSpec₁) :
     Verifier oSpec StmtIn StmtOut pSpec₂ where
-  verify := fun stmt transcript => V.verify stmt (dcast₂ h.symm (dcast_symm h hSpec) transcript)
+  verify := fun stmt transcript => V.verify stmt (dcast₂ hn.symm (dcast_symm hn hSpec) transcript)
 
 @[simp]
 theorem cast_id : Verifier.cast rfl rfl = (id : Verifier oSpec StmtIn StmtOut pSpec₁ → _) := by
@@ -202,9 +257,49 @@ instance instDCast₂Verifier :
   dcast₂_id := by intros; funext; simp
 
 theorem cast_eq_dcast₂ {V : Verifier oSpec StmtIn StmtOut pSpec₁} :
-    V.cast h hSpec = dcast₂ h hSpec V := rfl
+    V.cast hn hSpec = dcast₂ hn hSpec V := rfl
 
 end Verifier
+
+namespace OracleVerifier
+
+open OracleComp Function
+
+variable [∀ i, OracleInterface (pSpec₁.Message i)] [∀ i, OracleInterface (pSpec₂.Message i)]
+
+/-- Casting the oracle verifier of a non-oracle reduction across an equality of `ProtocolSpec`s.
+
+TODO: need a cast of the oracle interfaces as well (i.e. the oracle interface instance is not
+necessarily unique for every type) -/
+protected def cast (V : OracleVerifier oSpec StmtIn OStmtIn StmtOut OStmtOut pSpec₁) :
+    OracleVerifier oSpec StmtIn OStmtIn StmtOut OStmtOut pSpec₂ where
+  verify := fun stmt challenges =>
+    simulateQ sorry (V.verify stmt (dcast₂ hn.symm (dcast_symm hn hSpec) challenges))
+  embed := V.embed.trans
+    (Embedding.sumMap
+      (Equiv.refl _).toEmbedding
+      ⟨MessageIdx.cast hn hSpec, MessageIdx.cast_injective hn hSpec⟩)
+  hEq := fun i => by
+    simp [Embedding.sumMap, Equiv.refl]
+    have := V.hEq i
+    rw [this]
+    split
+    next a b h' => simp [h']
+    next a b h' => simp [h', MessageIdx.cast]; congr; exact (cast_idx hn hSpec).symm
+
+@[simp]
+theorem cast_id :
+    OracleVerifier.cast rfl rfl =
+      (id : OracleVerifier oSpec StmtIn OStmtIn StmtOut OStmtOut pSpec₁ → _) := by
+  sorry
+
+-- Need to cast oracle interface as well
+-- instance instDCast₂OracleVerifier : DCast₃ Nat ProtocolSpec
+--     (fun _ pSpec => OracleVerifier oSpec StmtIn OStmtIn StmtOut OStmtOut pSpec) where
+--   dcast₂ := OracleVerifier.cast
+--   dcast₂_id := OracleVerifier.cast_id
+
+end OracleVerifier
 
 namespace Reduction
 
@@ -212,18 +307,44 @@ namespace Reduction
   casts the underlying prover and verifier. -/
 protected def cast (R : Reduction oSpec StmtIn WitIn StmtOut WitOut pSpec₁) :
     Reduction oSpec StmtIn WitIn StmtOut WitOut pSpec₂ where
-  prover := R.prover.cast h hSpec
-  verifier := R.verifier.cast h hSpec
+  prover := R.prover.cast hn hSpec
+  verifier := R.verifier.cast hn hSpec
 
 @[simp]
-def cast_id {R : Reduction oSpec StmtIn WitIn StmtOut WitOut pSpec₁} :
-      R.cast rfl rfl = R := by
-  ext : 1 <;> simp [Reduction.cast, Prover.cast, Verifier.cast]
-  rfl
+theorem cast_id :
+    Reduction.cast rfl rfl = (id : Reduction oSpec StmtIn WitIn StmtOut WitOut pSpec₁ → _) := by
+  funext; simp [Reduction.cast]
 
-instance instDCast₂Verifier :
-    DCast₂ Nat ProtocolSpec (fun _ pSpec => Verifier oSpec StmtIn StmtOut pSpec) where
-  dcast₂ := Verifier.cast
-  dcast₂_id := by intros; funext; simp
+instance instDCast₂Reduction :
+    DCast₂ Nat ProtocolSpec (fun _ pSpec => Reduction oSpec StmtIn WitIn StmtOut WitOut pSpec) where
+  dcast₂ := Reduction.cast
+  dcast₂_id := Reduction.cast_id
 
 end Reduction
+
+namespace OracleReduction
+
+variable [∀ i, OracleInterface (pSpec₁.Message i)] [∀ i, OracleInterface (pSpec₂.Message i)]
+
+/-- Casting the oracle reduction across an equality of `ProtocolSpec`s, which casts the underlying
+  prover and verifier. -/
+protected def cast (R : OracleReduction oSpec StmtIn OStmtIn WitIn StmtOut OStmtOut WitOut pSpec₁) :
+    OracleReduction oSpec StmtIn OStmtIn WitIn StmtOut OStmtOut WitOut pSpec₂ where
+  prover := R.prover.cast hn hSpec
+  verifier := R.verifier.cast hn hSpec
+
+@[simp]
+theorem cast_id :
+    OracleReduction.cast rfl rfl =
+      (id : OracleReduction oSpec StmtIn OStmtIn WitIn StmtOut OStmtOut WitOut pSpec₁ → _) := by
+  ext : 2 <;> simp [OracleReduction.cast]
+
+-- Need to cast oracle interface as well
+-- instance instDCast₂OracleReduction :
+--     DCast₂ Nat ProtocolSpec
+--     (fun _ pSpec => OracleReduction oSpec StmtIn OStmtIn WitIn StmtOut OStmtOut WitOut pSpec)
+-- where
+--   dcast₂ := OracleReduction.cast
+--   dcast₂_id := OracleReduction.cast_id
+
+end OracleReduction
